DS: defined+implemented DS.Sessions module

denning-sacco/DS.Sessions.fst
@@ -1,1 +1,55 @@
 module DS.Sessions
+
+
+let serialize_session_st i p si vi st =
+  match st with
+  | InitiatorSentMsg1 b srv ->
+    let tag = str_to_bytes #i "i_sent_m1" in
+    let b_bytes = str_to_bytes #i b in
+    let srv_bytes = str_to_bytes #i srv in
+    concat #i #(readers [V p si vi]) tag (concat #i #(readers [V p si vi]) b_bytes srv_bytes)
+  | AuthServerSentMsg2 a b ->
+    let tag = str_to_bytes #i "srv_sent_m2" in
+    let a_bytes = str_to_bytes #i a in
+    let b_bytes = str_to_bytes #i b in
+    concat #i #(readers [V p si vi]) tag (concat #i #(readers [V p si vi]) a_bytes b_bytes)
+  | InitiatorSentMsg3 b ck ->
+    let tag = str_to_bytes #i "i_sent_m3" in
+    let b_bytes = str_to_bytes #i b in
+    concat #i #(readers [V p si vi]) tag (concat #i #(readers [V p si vi]) b_bytes ck)
+  | ResponderRecvedMsg3 a ck ->
+    let tag = str_to_bytes #i "r_rcvd_m3" in
+    let a_bytes = str_to_bytes #i a in
+    LC.can_flow_transitive i (LC.get_label M.ds_key_usages ck) (readers [P p]) (readers [V p si vi]);
+    concat #i #(readers [V p si vi]) tag (concat #i #(readers [V p si vi]) a_bytes ck)
+
+let parse_session_st sst =
+  split sst `bind` (fun (tag_bytes, rest) ->
+  bytes_to_string tag_bytes `bind` (fun tag ->
+  match tag with
+  | "i_sent_m1" ->
+    split rest `bind` (fun (b_bytes, srv_bytes) ->
+    bytes_to_string b_bytes `bind` (fun b ->
+    bytes_to_string srv_bytes `bind` (fun srv ->
+    Success (InitiatorSentMsg1 b srv))))
+  | "srv_sent_m2" ->
+    split rest `bind` (fun (a_bytes, b_bytes) ->
+    bytes_to_string a_bytes `bind` (fun a ->
+    bytes_to_string b_bytes `bind` (fun b ->
+    Success (AuthServerSentMsg2 a b))))
+  | "i_sent_m3" ->
+    split rest `bind` (fun (b_bytes, ck) ->
+    bytes_to_string b_bytes `bind` (fun b ->
+    Success (InitiatorSentMsg3 b ck)))
+  | "r_rcvd_m3" ->
+    split rest `bind` (fun (a_bytes, ck) ->
+    bytes_to_string a_bytes `bind` (fun a ->
+    Success (ResponderRecvedMsg3 a ck)))
+  | t -> Error ("[parse_session_st] invalid tag: " ^ t)
+  ))
+
+let parse_serialize_session_st_lemma i p si vi st =
+  match st with
+  | ResponderRecvedMsg3 a ck ->
+    LC.can_flow_transitive i (LC.get_label M.ds_key_usages ck) (readers [P p]) (readers [V p si vi])
+  | _ -> ()
